The **commutator** of [[operator]] $\widehat{A}$ and $\widehat{B}$ measures the failure to commute.

$$
\left[ \widehat{A}, \widehat{B} \right] \equiv \widehat{A}\widehat{B} - \widehat{B}\widehat{A}
$$

# Identities

$$
\left[\widehat{A}, \widehat{B}\widehat{C}\right]\equiv\left[\widehat{A}, \widehat{B}\right]\widehat{C} + \widehat{B}\left[\widehat{A}, \widehat{C}\right]
$$

$$
\left[\widehat{A}\widehat{B}, \widehat{C}\right]\equiv \widehat{A}\left[\widehat{B}, \widehat{C}\right] + \left[\widehat{A}, \widehat{C}\right]\widehat{B}
$$

$$
\left[\widehat{A} + \widehat{B}, \widehat{C}\right] \equiv \left[ \widehat{A}, \widehat{C} \right] + \left[ \widehat{B}, \widehat{C} \right]
$$