\begin{equation}
R(\vartheta) = \begin{bmatrix}\cos \vartheta & -\sin\vartheta \\\ \sin\vartheta & \cos\vartheta
\end{bmatrix}
\end{equation}

**Proof**. Let $v = \langle \cos \alpha, \sin \alpha \rangle$. Then,

\begin{align}
R(\vartheta)v &= \begin{bmatrix}\cos \vartheta & -\sin\vartheta \\\ \sin\vartheta & \cos\vartheta
\end{bmatrix}\begin{bmatrix}\cos\alpha \\\ \sin\alpha\end{bmatrix} \\\
&= \begin{bmatrix}\cos\vartheta \cos\alpha - \sin\theta\sin\alpha \\\ \sin\vartheta\cos\alpha + \cos\theta\sin\alpha \end{bmatrix} \\\
&= \begin{bmatrix}\cos(\alpha+\vartheta) \\\ \sin(\alpha+\vartheta)\end{bmatrix}
\end{align}